Reorganize dag modules to enforce better abstraction
We still only enforce it in Symbolic.v, but hopefully that'll be enough
to mostly ensure that future changes to one dag representation don't
desync with the other one.

Hopefully at some point I or someone else will manage to track down the
performance issues in switching to the New dag representation, and then
maybe we'll be able to drop this?  Or it might be good to make it easy
to change dag representations in the future.

In doing this, I've taken the opportunity to deduplicate some proofs
between the new and old implementations.

src/Assembly/Symbolic.v
@@ -1043,31 +1043,24 @@ Proof. repeat intro; subst; assumption. Qed.
 Existing Class node_ok.
 #[global]
 Hint Extern 1 (node_ok ?i ?n) => exact (@new_node_ok n I i) : typeclass_instances.
-Module Old.
-Module dag.
-  Definition t : Type := list (node idx * description * option ZRange.zrange).
-  Definition empty : t := nil.
-  Definition size (d : t) : N := N.of_nat (List.length d).
-  Definition lookup (d : t) (i : idx) : option (node idx)
-    := option_map (fun '(n, _d, _b) => n) (List.nth_error d (N.to_nat i)).
-  Definition lookup_bounds (d : t) (i : idx) : option ZRange.zrange
-    := (n <- List.nth_error d (N.to_nat i); let '(_n, _d, b) := n in b)%option.
-  Definition reverse_lookup (d : t) (i : node idx) : option idx
-    := option_map N.of_nat (List.indexof (fun '(n', _, _) => node_beq N.eqb i n') d).
-  Definition size_ok (d : t) : Prop
-    := True.
+Module Type DagDefinitions.
+  Parameter t : Type.
+  Parameter empty : t.
+  Parameter size : t -> N.
+  Parameter lookup : t -> idx -> option (node idx).
+  Parameter lookup_bounds : t -> idx -> option ZRange.zrange.
+  Parameter reverse_lookup : t -> node idx -> option idx.
+  Axiom size_ok : t -> Prop.
+  Axiom merge_node : forall {descr : description} (n : node idx) (d : t), idx * t.
+End DagDefinitions.
+Module DagExtraDefinitions (Import dag : DagDefinitions).
   Definition all_nodes_ok (d : t) : Prop
     := forall i r, lookup d i = Some r -> node_ok i r.
   Definition ok (d : t) : Prop
   := size_ok d
      /\ (forall i n, reverse_lookup d n = Some i <-> lookup d i = Some n)
      /\ (forall i n, lookup d i = Some n -> (i < size d)%N).
-  Definition merge_node {descr : description} (n : node idx) (d : t) : idx * t
-    := match reverse_lookup d n with
-       | Some i => (i, d)
-       | None
-         => (size d, d ++ [(n, descr, bound_node_idx_via_PHOAS (lookup_bounds d) n)])
-       end.
+
   Definition gensym (s:OperationSize) (d : t) : node idx
     := (old s (size d), []).
   Existing Class ok.
@@ -1080,21 +1073,62 @@ Module dag.
   Definition force_description : description -> eager_description
     := option_map (fun '(descr, always_show) => (descr tt, always_show)).
 
-  Module eager.
-    Definition t := list (idx * node idx * eager_description).
-    Definition force (d : dag.t) : eager.t
-      := List.map (fun '(idx, (n, descr, _)) => (N.of_nat idx, n, force_description descr))
-                  (List.enumerate d).
-    Definition description_lookup (d : eager.t) (descr : string) : list idx
-      := List.map (fun '(idx, _, _) => idx) (List.filter (fun '(_, _, descr') => match get_eager_description_description descr' with Some descr' => String.eqb descr descr' | _ => false end) d).
-  End eager.
-
   Definition M T := t -> T * t.
   Definition bind {A B} (v : M A) (f : A -> M B) : M B
     := fun d => let '(v, d) := v d in f v d.
   Definition ret {A} (v : A) : M A
     := fun d => (v, d).
 
+  Module Type EagerDagDefinitions.
+    Parameter t : Type.
+    Parameter force : dag.t -> t.
+    Parameter description_lookup : forall (d : t) (descr : string), list idx.
+    Parameter elements : t -> list (idx * node idx * eager_description).
+  End EagerDagDefinitions.
+End DagExtraDefinitions.
+Module Type DagExtraDefinitionsSig (dag : DagDefinitions).
+  Include DagExtraDefinitions dag.
+End DagExtraDefinitionsSig.
+Module Type DagProperties (Import dag : DagDefinitions) (Import dag' : DagExtraDefinitionsSig dag).
+  Axiom lookup_merge_node
+    : forall {descr : description} (n : node idx) (d : t) i
+             {ok : ok d},
+      dag.lookup (snd (dag.merge_node n d)) i = match dag.lookup d i with
+                                                | Some v => Some v
+                                                | None
+                                                  => if (i =? size d)%N && Option.is_None (reverse_lookup d n)
+                                                     then Some n
+                                                     else None
+                                                end.
+
+  Axiom reverse_lookup_merge_node
+    : forall {d : t}
+             {ok : ok d} {descr : description} (n n' : node idx),
+      dag.reverse_lookup (snd (dag.merge_node n d)) n'
+      = if node_beq N.eqb n' n
+        then Some (fst (dag.merge_node n d))
+        else dag.reverse_lookup d n'.
+
+  Axiom fst_merge_node
+    : forall {descr : description} (n : node idx) (d : t),
+      fst (dag.merge_node n d) = match reverse_lookup d n with
+                                 | Some i => i
+                                 | None => size d
+                                 end.
+
+  Axiom lookup_empty : forall i, lookup empty i = None.
+  Axiom reverse_lookup_empty : forall n, reverse_lookup empty n = None.
+  Axiom size_empty : size empty = 0%N.
+  Axiom size_ok_empty : size_ok empty.
+
+  Axiom size_merge_node
+    : forall {descr:description} n (d:t),
+      size (snd (merge_node n d)) = match reverse_lookup d n with Some _ => size d | None => N.succ (size d) end.
+  Axiom size_ok_merge_node
+    : forall {descr:description} n (d:t),
+      ok d -> size_ok (snd (merge_node n d)).
+End DagProperties.
+Module DagExtraProperties (Import dag : DagDefinitions) (Import dag' : DagExtraDefinitionsSig dag) (Import dag'' : DagProperties dag dag').
   Lemma iff_reverse_lookup_lookup d {ok : ok d}
     : forall i n, reverse_lookup d n = Some i <-> lookup d i = Some n.
   Proof. apply ok. Qed.
@@ -1110,6 +1144,173 @@ Module dag.
     specialize_under_binders_by reflexivity.
     lia.
   Qed.
+
+  Lemma reverse_lookup_gensym s (d : t)
+        {ok : ok d}
+        {all_nodes_ok : all_nodes_ok d}
+    : dag.reverse_lookup d (gensym s d) = None.
+  Proof.
+    cbv [dag'.all_nodes_ok] in *.
+    destruct (reverse_lookup d (gensym s d)) as [i|] eqn:H; [ | reflexivity ].
+    rewrite iff_reverse_lookup_lookup in H by assumption.
+    cbv [node_ok gensym] in *.
+    specialize_under_binders_by eassumption.
+    specialize_under_binders_by reflexivity.
+    apply lookup_value_size in H; trivial.
+    lia.
+  Qed.
+
+  Lemma lookup_merge_node_gensym {descr : description} s (d : t) i
+        {ok : ok d}
+        {all_nodes_ok : all_nodes_ok d}
+    : dag.lookup (snd (dag.merge_node (gensym s d) d)) i
+      = if (i =? size d)%N
+        then Some (gensym s d)
+        else dag.lookup d i.
+  Proof.
+    rewrite lookup_merge_node, reverse_lookup_gensym by assumption.
+    cbv [andb is_None].
+    break_innermost_match; try reflexivity; reflect_hyps; subst; try tauto.
+    rewrite lookup_size_error in * by first [ assumption | lia ].
+    congruence.
+  Qed.
+
+  Lemma fst_merge_node_gensym {descr : description} s (d : t)
+        {ok : ok d}
+        {all_nodes_ok : all_nodes_ok d}
+    : fst (dag.merge_node (gensym s d) d) = size d.
+  Proof.
+    rewrite fst_merge_node, reverse_lookup_gensym by assumption; reflexivity.
+  Qed.
+
+  Lemma size_merge_node_le {descr:description} n (d:t)
+    : (size d <= size (snd (merge_node n d)))%N.
+  Proof.
+    rewrite size_merge_node; break_innermost_match; lia.
+  Qed.
+
+  Lemma size_merge_node_gensym {descr:description} s (d:t)
+        {ok : ok d}
+        {all_nodes_ok : all_nodes_ok d}
+    : size (snd (merge_node (gensym s d) d)) = N.succ (size d).
+  Proof. rewrite size_merge_node, reverse_lookup_gensym by assumption; reflexivity. Qed.
+
+  Global Instance empty_ok : ok empty | 10.
+  Proof.
+    repeat apply conj; intros *;
+      rewrite ?lookup_empty, ?reverse_lookup_empty; try apply size_ok_empty;
+      intuition congruence.
+  Qed.
+  Global Instance empty_all_nodes_ok : all_nodes_ok empty | 10.
+  Proof.
+    repeat intro; subst; rewrite lookup_empty in *; congruence.
+  Qed.
+  Global Instance merge_node_ok {descr:description} {n:node idx} {d : t} {dok : ok d} : ok (snd (merge_node n d)) | 10.
+  Proof.
+    destruct (dok).
+    repeat apply conj; intros *.
+    all: rewrite ?lookup_merge_node, ?reverse_lookup_merge_node, ?fst_merge_node, ?size_merge_node by assumption.
+    all: let tac :=
+           repeat first [ progress subst
+                        | progress intros
+                        | progress destruct_head'_and
+                        | progress reflect_hyps
+                        | break_innermost_match_step
+                        | break_innermost_match_hyps_step
+                        | apply size_ok_merge_node
+                        | lia
+                        | progress inversion_option
+                        | progress specialize_under_binders_by reflexivity
+                        | congruence
+                        | tauto
+                        | match goal with
+                          | [ H : lookup ?d (size ?d) = Some _ |- _ ] => apply lookup_value_size in H; [ | assumption .. ]
+                          end
+                        | split
+                        | progress split_iff ] in
+         do 2 (tac;
+               repeat match goal with
+                      | [ H : _ = Some _ |- _ ] => progress specialize_all_ways_under_binders_by rewrite H
+                      end;
+               tac).
+  Qed.
+  Global Instance merge_node_all_nodes_ok {descr:description} {n:node idx} {d : t} {dok : ok d} {dnok : all_nodes_ok d} {nok : node_ok (size d) n}
+    : all_nodes_ok (snd (merge_node n d)) | 10.
+  Proof.
+    cbv [all_nodes_ok] in *; intros i r; specialize (dnok i r).
+    rewrite lookup_merge_node in * by assumption.
+    cbv [andb is_None]; break_innermost_match; intros; inversion_option; reflect_hyps; subst; auto.
+  Qed.
+  Global Instance gensym_node_ok s d : node_ok (size d) (gensym s d) | 10.
+  Proof.
+    cbv [node_ok]; intros * H.
+    inversion H; subst; reflexivity.
+  Qed.
+  Global Hint Extern 1 (node_ok (size _) (gensym _ _)) => exact (@gensym_node_ok _ _) : typeclass_instances.
+
+  Lemma eq_fst_merge_node_change_descr {descr1 descr2 : description} (n : node idx) (d : t)
+    : fst (@merge_node descr1 n d) = fst (@merge_node descr2 n d).
+  Proof.
+    rewrite !fst_merge_node; reflexivity.
+  Qed.
+
+  Lemma lookup_merge_node' {descr1 descr2 : description} (n : node idx) (d : t)
+        {ok : ok d}
+    : dag.lookup (snd (@dag.merge_node descr1 n d)) (fst (@dag.merge_node descr2 n d)) = Some n.
+  Proof.
+    rewrite lookup_merge_node, fst_merge_node by assumption.
+    cbv [andb is_None].
+    repeat first [ rewrite iff_reverse_lookup_lookup in * by assumption
+                 | rewrite lookup_size_error in * by first [ assumption | lia ]
+                 | progress inversion_option
+                 | progress subst
+                 | reflexivity
+                 | progress reflect_hyps
+                 | lia
+                 | break_innermost_match_step ].
+  Qed.
+End DagExtraProperties.
+Module Type DagExtraPropertiesSig (dag : DagDefinitions) (dag' : DagExtraDefinitionsSig dag) (dag'' : DagProperties dag dag').
+  Include DagExtraProperties dag dag' dag''.
+End DagExtraPropertiesSig.
+Module Type Dag.
+  Include DagDefinitions.
+  Include DagExtraDefinitions.
+  Declare Module eager : EagerDagDefinitions.
+  Include DagProperties.
+  Include DagExtraProperties.
+End Dag.
+Module Old.
+Module dag <: Dag.
+  Definition t : Type := list (node idx * description * option ZRange.zrange).
+  Definition empty : t := nil.
+  Definition size (d : t) : N := N.of_nat (List.length d).
+  Definition lookup (d : t) (i : idx) : option (node idx)
+    := option_map (fun '(n, _d, _b) => n) (List.nth_error d (N.to_nat i)).
+  Definition lookup_bounds (d : t) (i : idx) : option ZRange.zrange
+    := (n <- List.nth_error d (N.to_nat i); let '(_n, _d, b) := n in b)%option.
+  Definition reverse_lookup (d : t) (i : node idx) : option idx
+    := option_map N.of_nat (List.indexof (fun '(n', _, _) => node_beq N.eqb i n') d).
+  Definition size_ok (d : t) : Prop
+    := True.
+  Definition merge_node {descr : description} (n : node idx) (d : t) : idx * t
+    := match reverse_lookup d n with
+       | Some i => (i, d)
+       | None
+         => (size d, d ++ [(n, descr, bound_node_idx_via_PHOAS (lookup_bounds d) n)])
+       end.
+
+  Include DagExtraDefinitions.
+
+  Module eager <: EagerDagDefinitions.
+    Definition t := list (idx * node idx * eager_description).
+    Definition force (d : dag.t) : eager.t
+      := List.map (fun '(idx, (n, descr, _)) => (N.of_nat idx, n, force_description descr))
+                  (List.enumerate d).
+    Definition description_lookup (d : eager.t) (descr : string) : list idx
+      := List.map (fun '(idx, _, _) => idx) (List.filter (fun '(_, _, descr') => match get_eager_description_description descr' with Some descr' => String.eqb descr descr' | _ => false end) d).
+    Definition elements (d : t) : list (idx * node idx * eager_description) := d.
+  End eager.
 
   Lemma lookup_merge_node {descr : description} (n : node idx) (d : t) i
         {ok : ok d}
@@ -1177,50 +1378,14 @@ Module dag.
                                  end.
   Proof. cbv [merge_node]; break_innermost_match; reflexivity. Qed.
 
-  Lemma reverse_lookup_gensym s (d : t)
-        {ok : ok d}
-        {all_nodes_ok : all_nodes_ok d}
-    : dag.reverse_lookup d (gensym s d) = None.
-  Proof.
-    cbv [dag.all_nodes_ok] in *.
-    destruct (reverse_lookup d (gensym s d)) as [i|] eqn:H; [ | reflexivity ].
-    rewrite iff_reverse_lookup_lookup in H by assumption.
-    cbv [node_ok gensym] in *.
-    specialize_under_binders_by eassumption.
-    specialize_under_binders_by reflexivity.
-    apply lookup_value_size in H; trivial.
-    lia.
-  Qed.
-
-  Lemma lookup_merge_node_gensym {descr : description} s (d : t) i
-        {ok : ok d}
-        {all_nodes_ok : all_nodes_ok d}
-    : dag.lookup (snd (dag.merge_node (gensym s d) d)) i
-      = if (i =? size d)%N
-        then Some (gensym s d)
-        else dag.lookup d i.
-  Proof.
-    rewrite lookup_merge_node, reverse_lookup_gensym by assumption.
-    cbv [andb is_None].
-    break_innermost_match; try reflexivity; reflect_hyps; subst; try tauto.
-    rewrite lookup_size_error in * by first [ assumption | lia ].
-    congruence.
-  Qed.
-
-  Lemma fst_merge_node_gensym {descr : description} s (d : t)
-        {ok : ok d}
-        {all_nodes_ok : all_nodes_ok d}
-    : fst (dag.merge_node (gensym s d) d) = size d.
-  Proof.
-    rewrite fst_merge_node, reverse_lookup_gensym by assumption; reflexivity.
-  Qed.
-
   Lemma lookup_empty i : lookup empty i = None.
   Proof. cbv [empty lookup]; now rewrite nth_error_nil_error. Qed.
   Lemma reverse_lookup_empty n : reverse_lookup empty n = None.
   Proof. reflexivity. Qed.
   Lemma size_empty : size empty = 0%N.
   Proof. reflexivity. Qed.
+  Lemma size_ok_empty : size_ok empty.
+  Proof. exact I. Qed.
 
   Lemma size_merge_node {descr:description} n (d:t)
     : size (snd (merge_node n d)) = match reverse_lookup d n with Some _ => size d | None => N.succ (size d) end.
@@ -1228,119 +1393,15 @@ Module dag.
     cbv [merge_node size]; break_innermost_match; cbn [snd] in *; inversion_pair; subst; rewrite ?app_length; cbn [List.length]; lia.
   Qed.
 
-  Lemma size_merge_node_le {descr:description} n (d:t)
-    : (size d <= size (snd (merge_node n d)))%N.
-  Proof.
-    rewrite size_merge_node; break_innermost_match; lia.
-  Qed.
+  Lemma size_ok_merge_node {descr:description} n (d:t)
+    : ok d -> size_ok (snd (merge_node n d)).
+  Proof. constructor. Qed.
 
-  Lemma size_merge_node_gensym {descr:description} s (d:t)
-        {ok : ok d}
-        {all_nodes_ok : all_nodes_ok d}
-    : size (snd (merge_node (gensym s d) d)) = N.succ (size d).
-  Proof. rewrite size_merge_node, reverse_lookup_gensym by assumption; reflexivity. Qed.
-
-  Global Instance empty_ok : ok empty | 10.
-  Proof.
-    repeat apply conj; cbv [size empty]; intros *; cbv [lookup];
-      rewrite ?nth_error_nil_error; cbn; try exact I;
-      intuition first [ congruence | lia ].
-  Qed.
-  Global Instance empty_all_nodes_ok : all_nodes_ok empty | 10.
-  Proof.
-    repeat intro; subst; rewrite lookup_empty in *; congruence.
-  Qed.
-  Global Instance merge_node_ok {descr:description} {n:node idx} {d : t} {dok : ok d} : ok (snd (merge_node n d)) | 10.
-  Proof.
-    repeat apply conj; cbv [size empty size_ok]; intros *.
-    all: rewrite ?lookup_merge_node, ?reverse_lookup_merge_node by assumption.
-    all: let tac :=
-           repeat first [ progress cbv [ok size_ok size merge_node lookup reverse_lookup lookup_bounds Crypto.Util.Option.bind] in *
-                        | progress destruct_head'_and
-                        | progress inversion_option
-                        | progress subst
-                        | exfalso; assumption
-                        | progress inversion_pair
-                        | progress cbn [fst snd List.length List.app] in *
-                        | break_innermost_match_step
-                        | progress intros
-                        | progress destruct_head'_ex
-                        | progress destruct_head'_and
-                        | progress reflect_hyps
-                        | progress split_iff
-                        | apply conj
-                        | exact I
-                        | progress cbv [option_map idx] in *
-                        | progress break_match
-                        | progress break_match_hyps
-                        | lia
-                        | congruence
-                        | rewrite Nat2N.id in *
-                        | rewrite N2Nat.id in *
-                        | rewrite app_length
-                        | rewrite nth_error_app in *
-                        | progress specialize_under_binders_by reflexivity
-                        | progress specialize_under_binders_by rewrite Nat2N.id
-                        | progress destruct_head'_prod
-                        | progress inversion_list
-                        | match goal with
-                          | [ H : forall i n, match nth_error _ (N.to_nat i) with _ => _ end = _ -> _ |- _ ]
-                            => specialize (fun i => H (N.of_nat i))
-                          | [ H : _ = Some _ |- _ ] => rewrite H in *
-                          | [ H : N.of_nat _ = N.of_nat _ |- _ ] => apply (f_equal N.to_nat) in H
-                          | [ H : nth_error (_ :: _) _ = Some _ |- _ ]
-                            => apply nth_error_split in H
-                          | [ H : _ :: _ = ?x ++ _ |- _ ] => is_var x; destruct x
-                          | [ H : ?x ++ _ = nil |- _ ] => is_var x; destruct x
-                          | [ H : _ :: _ = _ :: _ |- _ ] => apply list_leq_to_eq in H; cbn [list_eq] in H
-                          end
-                        | solve [ exfalso; auto ] ] in
-         tac;
-         repeat match goal with
-                | [ H : _ = Some _ |- _ ] => progress specialize_all_ways_under_binders_by rewrite H
-                end;
-         tac.
-  Qed.
-  Global Instance merge_node_all_nodes_ok {descr:description} {n:node idx} {d : t} {dok : ok d} {dnok : all_nodes_ok d} {nok : node_ok (size d) n}
-    : all_nodes_ok (snd (merge_node n d)) | 10.
-  Proof.
-    cbv [all_nodes_ok] in *; intros i r; specialize (dnok i r).
-    rewrite lookup_merge_node in * by assumption.
-    cbv [andb is_None]; break_innermost_match; intros; inversion_option; reflect_hyps; subst; auto.
-  Qed.
-  Global Instance gensym_node_ok s d : node_ok (size d) (gensym s d) | 10.
-  Proof.
-    cbv [node_ok]; intros * H.
-    inversion H; subst; reflexivity.
-  Qed.
-  Global Hint Extern 1 (node_ok (size _) (gensym _ _)) => exact (@gensym_node_ok _ _) : typeclass_instances.
-
-  Lemma eq_fst_merge_node_change_descr {descr1 descr2 : description} (n : node idx) (d : t)
-    : fst (@merge_node descr1 n d) = fst (@merge_node descr2 n d).
-  Proof.
-    cbv [merge_node]; break_innermost_match; reflexivity.
-  Qed.
-
-  (* lemmas below here don't unfold the definitions *)
-  Lemma lookup_merge_node' {descr1 descr2 : description} (n : node idx) (d : t)
-        {ok : ok d}
-    : dag.lookup (snd (@dag.merge_node descr1 n d)) (fst (@dag.merge_node descr2 n d)) = Some n.
-  Proof.
-    rewrite lookup_merge_node, fst_merge_node by assumption.
-    cbv [andb is_None].
-    repeat first [ rewrite iff_reverse_lookup_lookup in * by assumption
-                 | rewrite lookup_size_error in * by first [ assumption | lia ]
-                 | progress inversion_option
-                 | progress subst
-                 | reflexivity
-                 | progress reflect_hyps
-                 | lia
-                 | break_innermost_match_step ].
-  Qed.
+  Include DagExtraProperties.
 End dag.
 End Old.
 Module New.
-Module dag.
+Module dag <: Dag.
   Module IdxMap <: UsualS := NMap <+ FMapFacts.Facts <+ Facts_RemoveHints <+ FMapFacts.AdditionalFacts.
   Module ListIdxMap <: UsualS := ListNMap.
   Module NodeIdxMap <: UsualS := ProdUsualMap OpMap ListIdxMap <+ FMapFacts.Facts <+ Facts_RemoveHints <+ FMapFacts.AdditionalFacts.
@@ -1360,12 +1421,6 @@ Module dag.
     := let '(im, nm, n) := d in
        NodeIdxMap.cardinal im = N.to_nat (size d)
        /\ IdxMap.cardinal nm = N.to_nat (size d).
-  Definition all_nodes_ok (d : t) : Prop
-    := forall i r, lookup d i = Some r -> node_ok i r.
-  Definition ok (d : t) : Prop
-  := size_ok d
-     /\ (forall i n, reverse_lookup d n = Some i <-> lookup d i = Some n)
-     /\ (forall i n, lookup d i = Some n -> (i < size d)%N).
   Definition merge_node {descr : description} (n : node idx) (d : t) : idx * t
     := match reverse_lookup d n with
        | Some i => (i, d)
@@ -1374,48 +1429,18 @@ Module dag.
             let '(d, d', sz) := d in
             (sz, (NodeIdxMap.add n sz d, IdxMap.add sz (n, descr, bound_node_idx_via_PHOAS lookup_bounds n) d', N.succ sz))
        end.
-  Definition gensym (s:OperationSize) (d : t) : node idx
-    := (old s (size d), []).
-  Existing Class ok.
-  Existing Class all_nodes_ok.
 
-  Definition get_eager_description_description (d : eager_description) : option string
-    := option_map fst d.
-  Definition get_eager_description_always_show (d : eager_description) : bool
-    := match d with Some (_, always_show) => always_show | None => false end.
-  Definition force_description : description -> eager_description
-    := option_map (fun '(descr, always_show) => (descr tt, always_show)).
+  Include DagExtraDefinitions.
 
-  Module eager.
+  Module eager <: EagerDagDefinitions.
     Definition t := list (idx * node idx * eager_description).
     Definition force (d : dag.t) : eager.t
       := List.map (fun '(idx, (n, descr, _b)) => (idx, n, force_description descr))
                   (IdxMap.elements (let '(_, d, _) := d in d)).
     Definition description_lookup (d : eager.t) (descr : string) : list idx
       := List.map (fun '(idx, _, _) => idx) (List.filter (fun '(_, _, descr') => match get_eager_description_description descr' with Some descr' => String.eqb descr descr' | _ => false end) d).
+    Definition elements (d : t) : list (idx * node idx * eager_description) := d.
   End eager.
-
-  Definition M T := t -> T * t.
-  Definition bind {A B} (v : M A) (f : A -> M B) : M B
-    := fun d => let '(v, d) := v d in f v d.
-  Definition ret {A} (v : A) : M A
-    := fun d => (v, d).
-
-  Lemma iff_reverse_lookup_lookup d {ok : ok d}
-    : forall i n, reverse_lookup d n = Some i <-> lookup d i = Some n.
-  Proof. apply ok. Qed.
-
-  Lemma lookup_value_size d {ok : ok d}
-    : forall i n, lookup d i = Some n -> (i < size d)%N.
-  Proof. apply ok. Qed.
-
-  Lemma lookup_size_error d {ok : ok d}
-    : forall i, (size d <= i)%N -> lookup d i = None.
-  Proof.
-    intro i; generalize (lookup_value_size d i); destruct lookup; intuition.
-    specialize_under_binders_by reflexivity.
-    lia.
-  Qed.
 
   Lemma lookup_merge_node {descr : description} (n : node idx) (d : t) i
         {ok : ok d}
@@ -1477,50 +1502,14 @@ Module dag.
                                  end.
   Proof. cbv [merge_node]; break_innermost_match; reflexivity. Qed.
 
-  Lemma reverse_lookup_gensym s (d : t)
-        {ok : ok d}
-        {all_nodes_ok : all_nodes_ok d}
-    : dag.reverse_lookup d (gensym s d) = None.
-  Proof.
-    cbv [dag.all_nodes_ok] in *.
-    destruct (reverse_lookup d (gensym s d)) as [i|] eqn:H; [ | reflexivity ].
-    rewrite iff_reverse_lookup_lookup in H by assumption.
-    cbv [node_ok gensym] in *.
-    specialize_under_binders_by eassumption.
-    specialize_under_binders_by reflexivity.
-    apply lookup_value_size in H; trivial.
-    lia.
-  Qed.
-
-  Lemma lookup_merge_node_gensym {descr : description} s (d : t) i
-        {ok : ok d}
-        {all_nodes_ok : all_nodes_ok d}
-    : dag.lookup (snd (dag.merge_node (gensym s d) d)) i
-      = if (i =? size d)%N
-        then Some (gensym s d)
-        else dag.lookup d i.
-  Proof.
-    rewrite lookup_merge_node, reverse_lookup_gensym by assumption.
-    cbv [andb is_None].
-    break_innermost_match; try reflexivity; reflect_hyps; subst; try tauto.
-    rewrite lookup_size_error in * by first [ assumption | lia ].
-    congruence.
-  Qed.
-
-  Lemma fst_merge_node_gensym {descr : description} s (d : t)
-        {ok : ok d}
-        {all_nodes_ok : all_nodes_ok d}
-    : fst (dag.merge_node (gensym s d) d) = size d.
-  Proof.
-    rewrite fst_merge_node, reverse_lookup_gensym by assumption; reflexivity.
-  Qed.
-
   Lemma lookup_empty i : lookup empty i = None.
   Proof. cbv [empty lookup]; now rewrite IdxMap.find_empty. Qed.
   Lemma reverse_lookup_empty n : reverse_lookup empty n = None.
   Proof. cbv [empty reverse_lookup]; now rewrite NodeIdxMap.find_empty. Qed.
   Lemma size_empty : size empty = 0%N.
   Proof. reflexivity. Qed.
+  Lemma size_ok_empty : size_ok empty.
+  Proof. cbv [size_ok empty size]; now rewrite NodeIdxMapProperties.P.cardinal_1, IdxMapProperties.P.cardinal_1 by first [ apply NodeIdxMap.empty_1 | apply IdxMap.empty_1 ]. Qed.
 
   Lemma size_merge_node {descr:description} n (d:t)
     : size (snd (merge_node n d)) = match reverse_lookup d n with Some _ => size d | None => N.succ (size d) end.
@@ -1528,101 +1517,30 @@ Module dag.
     cbv [merge_node size]; break_innermost_match; cbn [snd] in *; inversion_pair; subst; try reflexivity.
   Qed.
 
-  Lemma size_merge_node_le {descr:description} n (d:t)
-    : (size d <= size (snd (merge_node n d)))%N.
+  Lemma size_ok_merge_node {descr:description} n (d:t)
+    : ok d -> size_ok (snd (merge_node n d)).
   Proof.
-    rewrite size_merge_node; break_innermost_match; lia.
-  Qed.
-
-  Lemma size_merge_node_gensym {descr:description} s (d:t)
-        {ok : ok d}
-        {all_nodes_ok : all_nodes_ok d}
-    : size (snd (merge_node (gensym s d) d)) = N.succ (size d).
-  Proof. rewrite size_merge_node, reverse_lookup_gensym by assumption; reflexivity. Qed.
-
-  Global Instance empty_ok : ok empty | 10.
-  Proof.
-    repeat apply conj; cbv [size empty].
-    { apply NodeIdxMapProperties.P.cardinal_1, NodeIdxMap.empty_1. }
-    { apply IdxMapProperties.P.cardinal_1, IdxMap.empty_1. }
-    all: cbv [lookup reverse_lookup]; intros *.
-    all: rewrite ?NodeIdxMap.empty_o, ?IdxMap.empty_o; cbn; intuition congruence.
-  Qed.
-  Global Instance empty_all_nodes_ok : all_nodes_ok empty | 10.
-  Proof.
-    repeat intro; subst; rewrite lookup_empty in *; congruence.
-  Qed.
-  Global Instance merge_node_ok {descr:description} {n:node idx} {d : t} {dok : ok d} : ok (snd (merge_node n d)) | 10.
-  Proof.
-    repeat apply conj; cbv [size empty size_ok]; intros *.
-    all: rewrite ?lookup_merge_node, ?reverse_lookup_merge_node by assumption.
-    all: let tac :=
-           repeat first [ progress cbv [ok size_ok size merge_node lookup reverse_lookup option_map idx] in *
-                        | progress destruct_head'_and
-                        | progress inversion_option
-                        | progress subst
-                        | exfalso; assumption
-                        | progress inversion_pair
-                        | progress cbn [fst snd] in *
-                        | break_innermost_match_step
-                        | break_innermost_match_hyps_step
-                        | progress intros
-                        | progress reflect_hyps
-                        | progress split_iff
-                        | apply conj
-                        | rewrite NodeIdxMap.cardinal_add, NodeIdxMap.mem_find_b
-                        | rewrite IdxMap.cardinal_add, IdxMap.mem_find_b
-                        | rewrite N2Nat.inj_succ
-                        | lia
-                        | congruence
-                        | solve [ auto ]
-                        | match goal with
-                          | [ H : ?x = Some _ |- _ ] => rewrite H in *
-                          end
-                        | progress specialize_under_binders_by reflexivity ] in
-         tac;
-         specialize_all_ways;
-         tac.
-  Qed.
-  Global Instance merge_node_all_nodes_ok {descr:description} {n:node idx} {d : t} {dok : ok d} {dnok : all_nodes_ok d} {nok : node_ok (size d) n}
-    : all_nodes_ok (snd (merge_node n d)) | 10.
-  Proof.
-    cbv [all_nodes_ok] in *; intros i r; specialize (dnok i r).
-    rewrite lookup_merge_node in * by assumption.
-    cbv [andb is_None]; break_innermost_match; intros; inversion_option; reflect_hyps; subst; auto.
-  Qed.
-  Global Instance gensym_node_ok s d : node_ok (size d) (gensym s d) | 10.
-  Proof.
-    cbv [node_ok]; intros * H.
-    inversion H; subst; reflexivity.
-  Qed.
-  Global Hint Extern 1 (node_ok (size _) (gensym _ _)) => exact (@gensym_node_ok _ _) : typeclass_instances.
-
-  Lemma eq_fst_merge_node_change_descr {descr1 descr2 : description} (n : node idx) (d : t)
-    : fst (@merge_node descr1 n d) = fst (@merge_node descr2 n d).
-  Proof.
-    cbv [merge_node]; break_innermost_match; reflexivity.
-  Qed.
-
-  (* lemmas below here don't unfold the definitions *)
-  Lemma lookup_merge_node' {descr1 descr2 : description} (n : node idx) (d : t)
-        {ok : ok d}
-    : dag.lookup (snd (@dag.merge_node descr1 n d)) (fst (@dag.merge_node descr2 n d)) = Some n.
-  Proof.
-    rewrite lookup_merge_node, fst_merge_node by assumption.
-    cbv [andb is_None].
-    repeat first [ rewrite iff_reverse_lookup_lookup in * by assumption
-                 | rewrite lookup_size_error in * by first [ assumption | lia ]
-                 | progress inversion_option
-                 | progress subst
-                 | reflexivity
-                 | progress reflect_hyps
+    cbv [merge_node size_ok size ok]; break_innermost_match; cbn [snd] in *; inversion_pair; subst;
+      rewrite ?NodeIdxMap.cardinal_add, ?IdxMap.cardinal_add, ?NodeIdxMap.mem_find_b, ?IdxMap.mem_find_b; try solve [ intuition auto ]; [].
+    cbv [reverse_lookup lookup option_map idx] in *.
+    repeat first [ progress intros
+                 | progress destruct_head'_and
+                 | progress split_iff
+                 | congruence
                  | lia
-                 | break_innermost_match_step ].
+                 | break_innermost_match_step
+                 | break_innermost_match_hyps_step
+                 | progress specialize_under_binders_by reflexivity
+                 | match goal with
+                   | [ H : _ = Some _ |- _ ] => progress specialize_under_binders_by rewrite H
+                   end ].
   Qed.
+
+  Include DagExtraProperties.
 End dag.
 End New.
-Export Old.
+Require coqutil.Tactics.autoforward coqutil.Decidable coqutil.Tactics.Tactics.
+Module WithDag (dag : Dag).
 Global Arguments dag.t : simpl never.
 Global Arguments dag.empty : simpl never.
 Global Arguments dag.size : simpl never.
@@ -1938,7 +1856,7 @@ Proof using Type.
       | eauto using Forall2_weaken, eval_weaken_merge_node .. ]. }
 Qed.
 
-Require Import coqutil.Tactics.autoforward coqutil.Decidable coqutil.Tactics.Tactics.
+Import coqutil.Tactics.autoforward coqutil.Decidable coqutil.Tactics.Tactics.
 Global Set Default Goal Selector "1".
 
 Lemma eval_merge {descr:description} G :
@@ -2051,7 +1969,6 @@ Section bound_expr_via_PHOAS.
   Import AbstractInterpretation.ZRange.Compilers.
   Import AbstractInterpretation.ZRangeProofs.Compilers.
 
-  Local Instance : shiftr_avoid_uint1_opt := false.
   Local Notation interp_PHOAS_op := (ZRange.ident.option.interp true).
 
   Fixpoint bound_expr_via_PHOAS (d : dag) (e : Symbolic.expr) : option zrange
@@ -3719,7 +3636,7 @@ Global Instance show_lines_dag : ShowLines dag := (fun d:dag =>
                                                   | Some descr => " " ++ String.Tab ++ "(*" ++ descr ++ "*)"
                                                   | None => ""
                                                   end
-                                             else ""))%string (dag.eager.force d)
+                                             else ""))%string (dag.eager.elements (dag.eager.force d))
   ++["]"])%list%string.
 Global Instance show_lines_mem_state : ShowLines mem_state :=
   @show_lines_list _ ShowLines_of_Show.
@@ -4210,3 +4127,6 @@ Fixpoint SymexLines {opts : symbolic_options_computed_opt} (lines : Lines) : M u
        => (st <- SymexLine line;
           SymexLines lines)
      end.
+End WithDag.
+Export Old.
+Include WithDag dag.
